some progress

causal.v
@@ -2,50 +2,116 @@ Require Import Coq.Lists.List.
 Require Import Coq.Program.Basics.
 Require Import Coq.Logic.FunctionalExtensionality.
 
+(*|
+================================
+Transducers are Causal Functions
+================================
+
+|*)
+
+
+(*|
+Consider the set :math:`2^\omega` of infinite lists of natural numbers.
+
+What are the "nice" functions :math:`2^\omega \to 2^\omega`? 
+As indicated by the quotes, the answer to this question is highly dependent on your aesthetic preferences.
+Naturally, different people with different needs have proposed different answers based on a wide variety of values of "nice".
+
+One potential value of "nice" is the vacuous one: all (mathematically definable) functions :math:`2^\omega \to 2^\omega` are allowed!
+Among these are functions that aren't even definable as functions in your favorite programming language,
+such as the function :math:`f : 2^\omega \to 2^\omega` defined by :math:`f(1^\omega) = 0^\omega` and  :math:`f(s) = s`: the function
+which is the identity everywhere, except for on the stream of all ones, where it's the stream of all zeroes.
+This function is clearly not computable in any sense: in order to determine even the first element of the output stream,
+all infinitely-many elements of the input need to be inspected.
+
+Restricting "nice" to mean "computable" restricts the class significantly. Indeed, the main result is 
+the rule out functions like the one above. A classic result in computability theory is that the computable
+functions :math:`f : 2^\omega \to 2^\omega` are *continous* in a particular sense [#]_ which means that any finite prefix
+of the output of :math:`f` can only depend on a finite prefix of its input.
+
+However, the computable functions can include some unwanted behavior. Of particular interest for the purposes of this
+piece is functions that "go back on their word".
+A simple example of this is the function defined by the equations :math:`f(00s) = 01s`, :math:`f(01s) = 10s`, :math:`f(1s) = 1s`.
+To see why this might be undesierable, consider a situation where the input list to the function is being *streamed in*, bit by bit, from
+some outside source. Similarly, suppose the output is being produced bit by bit, and is fed to some similar transformation down the line.
+Unfortunately, the function :math:`f` cannot be implemented in this manner: if the first bit of input is a :math:`0`,
+the implementation must wait until the *second* bit arrives to emit the first bit of output. To faithfully implement this
+in such a "stream transformer" machine model, the machine would need the ability to either (a) block until the second bit arrives, or
+(b) emit a dummy value for the first output and then "retract" it once it got the second bit of input.
+
+Our goal in this **???* is to characterize the stream functions :math:`f : 2^\omega \to 2^\omega` which
+can be implemented as stream processing machines which are both (a) productive, in the sense that they always
+emit an output for each input, and (b) are *causal* in the sense that they
+
+
+|*)
+
 Variable A : Type.
 
-CoInductive autom : Type := 
-| Step : (A -> A * autom) -> autom.
+Coinductive stream : Type :=
+| SCons : A -> stream -> stream.
 
-Definition step (m : autom) (x : A) : A * autom :=
+(*|
+
+==========
+Transducer
+==========
+
+|*)
+
+
+CoInductive transd : Type := 
+| Step : (A -> A * transd) -> transd.
+
+Definition step (m : transd) (x : A) : A * transd :=
     match m with
     | Step f => f x
     end.
 
-Definition exec (m : autom) (x : A) : A :=
+
+Inductive listn : nat -> Type :=
+| Empty : listn 0
+| Snoc {n} : listn n -> A -> listn (S n).
+
+Fixpoint stepN {n} (m : transd) (l : listn n) : transd * listn n :=
+    match l with
+    | Empty => (m,Empty)
+    | Snoc l' x => let (m',l'') := stepN m l' in
+                              let (y,m'') := step m' x in
+                              (m'',Snoc l'' y)
+    end.
+
+Definition execN {n} (m : transd) (l : listn n) := snd (stepN m l).
+
+Definition exec (m : transd) (x : A) : A :=
     fst (step m x).
-
-Inductive lengthN : nat -> Type :=
-| Empty_lengthN : lengthN 0
-| Snoc_lengthN {n} : lengthN n -> A -> lengthN (S n).
-
-
-(* remove the first element *)
-Definition truncate {n : nat} (l : lengthN (S n)) : lengthN n := 
-  match l in lengthN (S n) return lengthN n with
-  | Snoc_lengthN l _ => l
-  end.
-
-
-Theorem trunc_0 : forall (l : lengthN 1), truncate l = Empty_lengthN.
-Proof.
-Admitted.
-
-Theorem lengthN_eta_0 : forall (l : lengthN 0), l = Empty_lengthN.
-Proof.
-Admitted.
-
-Theorem lengthN_eta_S : forall n, forall (l : lengthN (S n)), exists x , l = Snoc_lengthN (truncate l) x.
-Proof.
-Admitted.
-
 
 Record omega_presheaf : Type := mkPresheaf {
   fam : nat -> Type;
   restrict : forall n, fam (S n) -> fam n
 }.
 
-Definition lengthN_pshf : omega_presheaf := mkPresheaf lengthN (fun _ => truncate).
+
+(* remove the first element *)
+Definition truncate {n : nat} (l : listn (S n)) : listn n := 
+  match l in listn (S n) return listn n with
+  | Snoc l _ => l
+  end.
+
+
+Theorem trunc_0 : forall (l : listn 1), truncate l = Empty.
+Proof.
+Admitted.
+
+Theorem listn_eta_0 : forall (l : listn 0), l = Empty.
+Proof.
+Admitted.
+
+Theorem listn_eta_S : forall n, forall (l : listn (S n)), exists x , l = Snoc (truncate l) x.
+Proof.
+Admitted.
+
+Definition listn_pshf : omega_presheaf := mkPresheaf listn (fun _ => truncate).
 
 Record omega_presheaf_nt (P : omega_presheaf) (Q : omega_presheaf) : Type := mkNT {
   component : forall n, fam P n -> fam Q n;
@@ -73,22 +139,22 @@ Definition shiftNT {P Q} (alpha : omega_presheaf_nt P Q) : omega_presheaf_nt (sh
   mkNT (shift P) (shift Q) (shiftNT_component alpha) (shiftNT_squares alpha).
 
 
-Definition unshiftlengthNNT_component (alpha : omega_presheaf_nt (shift lengthN_pshf) (shift lengthN_pshf)) : forall n : nat, fam lengthN_pshf n -> fam lengthN_pshf n :=
+Definition unshiftlistnNT_component (alpha : omega_presheaf_nt (shift listn_pshf) (shift listn_pshf)) : forall n : nat, fam listn_pshf n -> fam listn_pshf n :=
     fun n => match n with
-             | 0 => fun _ => Empty_lengthN
-             | S n' => component (shift lengthN_pshf) (shift lengthN_pshf) alpha n'
+             | 0 => fun _ => Empty
+             | S n' => component (shift listn_pshf) (shift listn_pshf) alpha n'
     end.
 
-Theorem unshiftlengthNNT_squares (alpha : omega_presheaf_nt (shift lengthN_pshf) (shift lengthN_pshf)) : forall n : nat,
+Theorem unshiftlistnNT_squares (alpha : omega_presheaf_nt (shift listn_pshf) (shift listn_pshf)) : forall n : nat,
 compose
-  (unshiftlengthNNT_component alpha n)
-  (restrict lengthN_pshf n) =
-compose (restrict lengthN_pshf n)
-  (unshiftlengthNNT_component alpha (S n)).
+  (unshiftlistnNT_component alpha n)
+  (restrict listn_pshf n) =
+compose (restrict listn_pshf n)
+  (unshiftlistnNT_component alpha (S n)).
 Proof.
 simpl. induction n.
  - extensionality l. cbn. unfold compose. rewrite trunc_0. reflexivity.
- - simpl in *. apply (squares (shift lengthN_pshf) (shift lengthN_pshf) alpha).
+ - simpl in *. apply (squares (shift listn_pshf) (shift listn_pshf) alpha).
 Qed.
 
 (* There's a nice picture to draw here of the commutative diagrram: shiftNT pushes the indexing up by one, so
@@ -106,37 +172,29 @@ Qed.
 
    to get a full NT.
    This should probably work for any NT shift P => shift Q, by tainng a singleton set to be the zero component.
-   But this happens to be a lengthN_pshf anyway.
+   But this happens to be a listn_pshf anyway.
 *)
-Definition unshiftlengthNNT (alpha : omega_presheaf_nt (shift lengthN_pshf) (shift lengthN_pshf)) : omega_presheaf_nt lengthN_pshf lengthN_pshf :=
-    mkNT lengthN_pshf lengthN_pshf (unshiftlengthNNT_component alpha) (unshiftlengthNNT_squares alpha).
+Definition unshiftlistnNT (alpha : omega_presheaf_nt (shift listn_pshf) (shift listn_pshf)) : omega_presheaf_nt listn_pshf listn_pshf :=
+    mkNT listn_pshf listn_pshf (unshiftlistnNT_component alpha) (unshiftlistnNT_squares alpha).
 
-Definition len1Proj (x : fam lengthN_pshf 1) : A.
+Definition len1Proj (x : fam listn_pshf 1) : A.
 Proof.
 simpl in *. inversion x. apply X0.
 Qed.
 
-Definition headApply (alpha : omega_presheaf_nt lengthN_pshf lengthN_pshf) : A -> A :=
-  fun a => let l1 : fam lengthN_pshf 1 := Snoc_lengthN Empty_lengthN a in
-           let l2 : fam lengthN_pshf 1 := component _ _ alpha 1 l1 in
+Definition headApply (alpha : omega_presheaf_nt listn_pshf listn_pshf) : A -> A :=
+  fun a => let l1 : fam listn_pshf 1 := Snoc Empty a in
+           let l2 : fam listn_pshf 1 := component _ _ alpha 1 l1 in
            len1Proj l2.
 
-CoFixpoint fromNT (alpha : omega_presheaf_nt lengthN_pshf lengthN_pshf) : autom :=
-  Step (fun a => (headApply alpha a, fromNT (unshiftlengthNNT (shiftNT alpha)))).
+CoFixpoint fromNT (alpha : omega_presheaf_nt listn_pshf listn_pshf) : transd :=
+  Step (fun a => (headApply alpha a, fromNT (unshiftlistnNT (shiftNT alpha)))).
 
-Check lengthN_rec.
+Check listn_rec.
 
-Fixpoint stepN {n} (m : autom) (l : lengthN n) : autom * lengthN n :=
-    match l with
-    | Empty_lengthN => (m,Empty_lengthN)
-    | Snoc_lengthN l' x => let (m',l'') := stepN m l' in
-                              let (y,m'') := step m' x in
-                              (m'',Snoc_lengthN l'' y)
-    end.
 
-Definition execN {n} (m : autom) (l : lengthN n) := snd (stepN m l).
 
-Theorem exec_S : forall n m (l : lengthN n) x, exists y, (execN m (Snoc_lengthN l x) = Snoc_lengthN (execN m l) y).
+Theorem exec_S {n} : forall m (l : listn n) x, exists y, (execN m (Snoc l x) = Snoc (execN m l) y /\ (y = let (m',l') := stepN m l in fst (step m' x))).
 Proof.
   intros.
   exists (let (m',_) := stepN m l in fst (step m' x)).
@@ -145,31 +203,31 @@ Proof.
   destruct (stepN m l) as [m' l'].
   destruct (step m' x) as [y m''].
   cbn.
-  reflexivity.
+  auto.
 Qed.
 
-Theorem toNT_squares (m : autom) :
+Theorem toNT_squares (m : transd) :
   forall n : nat,
-   compose (execN m) (restrict lengthN_pshf n) =
-   compose (restrict lengthN_pshf n) (execN m).
+   compose (execN m) (restrict listn_pshf n) =
+   compose (restrict listn_pshf n) (execN m).
 Proof.
 intros.
 induction n.
 - simpl. extensionality l. unfold compose. rewrite trunc_0. simpl. rewrite trunc_0. reflexivity.
 - extensionality l. simpl in *. unfold compose in *.
-  assert (exists x , l = Snoc_lengthN (truncate l) x) by (apply lengthN_eta_S).
+  assert (exists x , l = Snoc (truncate l) x) by (apply listn_eta_S).
   destruct H.
   rewrite -> H.
   cbn.
-  assert (exists y, (execN m (Snoc_lengthN (truncate l) x) = Snoc_lengthN (execN m (truncate l)) y)) by (apply exec_S).
-  destruct H0 as [y HSnoc].
+  assert (exists y, (execN m (Snoc (truncate l) x) = Snoc (execN m (truncate l)) y) /\ _) by (apply exec_S).
+  destruct H0 as [y [HSnoc _]].
   rewrite -> HSnoc.
   cbn.
   reflexivity.
 Qed.
 
-Definition toNT (m : autom) : omega_presheaf_nt lengthN_pshf lengthN_pshf :=
-    mkNT lengthN_pshf lengthN_pshf (fun n => execN m) (toNT_squares m).
+Definition toNT (m : transd) : omega_presheaf_nt listn_pshf listn_pshf :=
+    mkNT listn_pshf listn_pshf (fun n => execN m) (toNT_squares m).
 
 (*
 * - Clear conception of who the audience is –– why do they care about this equivalence?
@@ -178,3 +236,15 @@ Definition toNT (m : autom) : omega_presheaf_nt lengthN_pshf lengthN_pshf :=
 * - Potentailly, an appenndix with thoughts on the process of turning the proof into a literate one.
 * - Ensure you have a trial reader!
 *)
+
+Theorem inv1 : forall alpha n, component _ _ (toNT (fromNT alpha)) n = component _ _ alpha n.
+Proof.
+  intros.
+  cbn.
+  extensionality l.
+Admitted.
+
+(*|
+.. [#] For the curious: by endowing :math:`2` with the discrete topology and :math:`2^\omega` with the product topology,
+the computable functions :math:`2^\omega \to 2^\omega` are continuous.
+|*)
